CBV -> CBPV Type Preservation Proof (#1)
* CBV translation preservation

* Share effects definition across CBPV/CBV

coq/CBV/cbv.sig
@@ -1,18 +1,13 @@
-type : Type
 bool : Type
 Value : Type
 Exp : Type
-
-Unit : type 
-Arr : type -> type -> type 
-Cross : type -> type -> type 
-Plus : type -> type -> type 
 
 One : Value
 Lam : (Value -> Exp) -> Value 
 Pair : Value -> Value -> Value 
 Inj: bool -> Value -> Value
 
+Tock : Exp
 Val : Value -> Exp 
 App : Exp -> Exp -> Exp 
 CaseS : Exp -> (Value -> Exp) -> (Value -> Exp) -> Exp
