coq/Effects.v
@@ -1,0 +1,48 @@
+
+Set Implicit Arguments.
+Require Import Psatz Logic List Classes.Morphisms.
+Import List Notations.
+
+Require Export Base.
+
+Parameter effect : Type.
+
+Parameter pure : effect.
+Parameter tick : effect.
+Parameter add : effect -> effect -> effect.
+
+(* Monoid laws *)
+
+Parameter eff_idL : forall {phi}, add pure phi = phi.
+Parameter eff_idR : forall {phi}, add phi pure = phi.
+Parameter eff_assoc : forall {phi1 phi2 phi3}, add (add phi1 phi2) phi3 = add phi1 (add phi2 phi3).
+
+#[export] Hint Resolve eff_idL eff_idR eff_assoc : core.
+#[export] Hint Rewrite @eff_idL @eff_idR @eff_assoc : core.
+
+(* Preordered monoid: preorder compatible with add *)
+
+Inductive subeff : effect -> effect -> Prop :=
+  | subeff_refl phi : subeff phi phi
+  | subeff_trans phi1 phi2 phi3 :
+    subeff phi1 phi2 -> subeff phi2 phi3 -> subeff phi1 phi3
+  | subeff_add_right_compatible phi1 phi2 phi :
+    subeff phi1 phi2 -> subeff (add phi1 phi) (add phi2 phi)
+  | subeff_add_left_compatible phi1 phi2 phi :
+    subeff phi1 phi2 -> subeff (add phi phi1) (add phi phi2).
+
+#[export] Hint Constructors subeff : core.
+
+Parameter subeff_pure : forall {phi}, subeff pure phi.
+
+Theorem subeff_addright : forall {phi1 phi2}, subeff phi1 (add phi1 phi2).
+Proof.
+  intros. rewrite <- eff_idR at 1. apply subeff_add_left_compatible. apply subeff_pure.
+Qed.
+
+Theorem subeff_addleft : forall {phi1 phi2}, subeff phi1 (add phi2 phi1).
+Proof.
+  intros. rewrite <- eff_idL at 1. apply subeff_add_right_compatible. apply subeff_pure.
+Qed.
+
+#[export] Hint Resolve subeff_addright subeff_addleft.
